rbt_insert

clrs/rbt_insert_gen.rkt
@@ -2,7 +2,8 @@
 (require "rbt_insert_inner_gen.rkt" "rbt_blacken_gen.rkt")
 
 (Fixpoint
- rbt_insert #:implicit @A{Set}
+ rbt_insert
+ @A{Set}
  @A_cmp{A -> A -> Prop}
  @A_refl{forall x, A_cmp x x}
  @A_asym{forall x y, A_cmp x y -> ~ A_cmp y x}
@@ -13,7 +14,7 @@
  @ct{CTree A} @x{A}
  #:returns @{CTree A}
  (bind 
-  ((ctp (rbt_insert_inner A_cmp A_refl A_asym A_trans A_cmp_dec A_eq_dec ct x)))
+  ((ctp (rbt_insert_inner A A_cmp A_refl A_asym A_trans A_cmp_dec A_eq_dec ct x)))
   (bind 
-   ((res (rbt_blacken ct)))
+   ((res (rbt_blacken A ctp)))
    (<== res))))
